simplify translate

Translation/Global.lean
@@ -5,47 +5,28 @@ import Surface.Typing
 
 import Translation.Ty
 
--- def Core.is_valid_ctor_ty (G : Core.GlobalEnv) : Core.Ty -> Option String
--- | .all _ T => is_valid_ctor_ty G T
--- | .arrow _ T => is_valid_ctor_ty G T
--- | t => do let (x, _) <- t.spine
---           if Core.is_data G x then return x else none
-
-
--- def Surface.is_valid_ctor_ty (G : Surface.GlobalEnv) : Surface.Ty -> Option String
--- | .all _ T => is_valid_ctor_ty G T
--- | .arrow _ T => is_valid_ctor_ty G T
--- | t => do let (x, _) <- t.spine
---           if Surface.is_data G x then return x else none
-
 
 def Surface.Ty.translate_ctors (ctors : Vect n (String × Surface.Ty)) : (Vect n (String × Core.Ty)) :=
   (λ (x, ty) => (x , ty.translate)) <$> ctors
 
--- def Core.Ty.check_ctor_tys (dx : String) (G : Core.GlobalEnv) (ctors : Vect n (String × Core.Ty)) : Option Unit := do
---   let check : Vect n (Option String) :=
---       (λ c => Core.is_valid_ctor_ty  G c.2) <$> ctors
---   let check' <- check.seq
---   -- TODO: check that names are unique
---   -- let cns : Vect n String := (λ x => x.1) <$> ctors
---   if check'.elems_eq_to dx then return () else none
-
-
 
 @[simp]
-def Surface.Global.translate (G : Core.GlobalEnv) : Global -> Option Core.Global
-| .data (n := n) x K ctors => do
+def Surface.Global.translate : Global -> Core.Global
+| .data (n := n) x K ctors =>
   let ctors' := Ty.translate_ctors ctors
   -- Core.Ty.check_ctor_tys x (.data 0 x K.translate Vect.nil :: G) ctors'
-  return Core.Global.data n x K.translate ctors'
+  Core.Global.data n x K.translate ctors'
 
 @[simp]
-def Surface.GlobalEnv.translate : Surface.GlobalEnv -> Option (Core.GlobalEnv)
-| [] => return []
+def Surface.GlobalEnv.translate : Surface.GlobalEnv -> Core.GlobalEnv
+| [] => []
 | .cons g gs => do
-  let gs' <- Surface.GlobalEnv.translate gs
-  let g' <- g.translate gs'
-  return g' :: gs'
+  let gs' := Surface.GlobalEnv.translate gs
+  let g' := g.translate
+  g' :: gs'
+
+-- def Surface.Entry.translate : Surface.Entry -> Option
+
 
 namespace Test.Core.Global
 
